src/compiler_generic/toy_example/embedding/meta_toy/Printer_Toy_extended.thy
@@ -103,9 +103,9 @@ definition "of_toy_def_state _ (floor :: (* polymorphism weakening needed by cod
 definition "of_toy_def_pp_core = (\<lambda> ToyDefPPCoreBinding s \<Rightarrow> To_string s
                                   | ToyDefPPCoreAdd l \<Rightarrow> \<open>[ %s ]\<close> (of_toy_def_state_core l))"
 
-definition "of_toy_def_pre_post _ (floor :: (* polymorphism weakening needed by code_reflect *)
+definition "of_toy_def_transition _ (floor :: (* polymorphism weakening needed by code_reflect *)
                                             String.literal) = (\<lambda> ToyDefPP n s_pre s_post \<Rightarrow>
-  \<open>PrePost%s %s%s%s\<close>
+  \<open>Transition%s %s%s%s\<close>
     floor
     (case n of None \<Rightarrow> \<open>\<close> | Some n \<Rightarrow> \<open>%s = \<close> (To_string n))
     (of_toy_def_pp_core s_pre)
@@ -122,7 +122,7 @@ lemmas [code] =
   Print.of_toy_def_state_core_def
   Print.of_toy_def_state_def
   Print.of_toy_def_pp_core_def
-  Print.of_toy_def_pre_post_def
+  Print.of_toy_def_transition_def
 
   (* fun *)
   Print.of_toy_list_attr.simps
