examples/archive/Flight_Model_compact.thy
@@ -256,11 +256,10 @@ where the latter only means that $X$'s object id exists both in $\sigma_1$ and
 $\sigma_2$, not that its content has not been changed.
 *}
 
-(* TODO : Rename PrePost into : Transition *)
-PrePost \<sigma>\<^sub>1 \<sigma>\<^sub>2
+Transition \<sigma>\<^sub>1 \<sigma>\<^sub>2
 
 
-locale TRANS_\<sigma>\<^sub>1_\<sigma>\<^sub>2
+locale TRANSITION_\<sigma>\<^sub>1_\<sigma>\<^sub>2
 begin
 lemma \<sigma>\<^sub>1: "state_interpretation_\<sigma>\<^sub>1 \<tau>"
 by(simp add: state_interpretation_\<sigma>\<^sub>1_def,
@@ -283,38 +282,38 @@ by(simp add: pp_\<sigma>\<^sub>1_\<sigma>\<^sub>2_def,
 
 definition \<sigma>\<^sub>0 :: "\<AA> state" where "\<sigma>\<^sub>0 = state.make Map.empty Map.empty"
 
-definition "\<sigma>\<^sub>1 = pre_post_\<sigma>\<^sub>1_\<sigma>\<^sub>2.\<sigma>\<^sub>1 oid3 oid4 oid5 oid6 oid7 oid8 oid9
+definition "\<sigma>\<^sub>t\<^sub>1 = transition_\<sigma>\<^sub>1_\<sigma>\<^sub>2.\<sigma>\<^sub>1 oid3 oid4 oid5 oid6 oid7 oid8 oid9
                   \<lceil>\<lceil>S1 (\<sigma>\<^sub>0, \<sigma>\<^sub>0)\<rceil>\<rceil> \<lceil>\<lceil>C1 (\<sigma>\<^sub>0, \<sigma>\<^sub>0)\<rceil>\<rceil> \<lceil>\<lceil>C2 (\<sigma>\<^sub>0, \<sigma>\<^sub>0)\<rceil>\<rceil> \<lceil>\<lceil>R11 (\<sigma>\<^sub>0, \<sigma>\<^sub>0)\<rceil>\<rceil>
                   \<lceil>\<lceil>R21 (\<sigma>\<^sub>0, \<sigma>\<^sub>0)\<rceil>\<rceil> \<lceil>\<lceil>F1 (\<sigma>\<^sub>0, \<sigma>\<^sub>0)\<rceil>\<rceil> \<lceil>\<lceil>F2 (\<sigma>\<^sub>0, \<sigma>\<^sub>0)\<rceil>\<rceil>"
 
-definition "\<sigma>\<^sub>2 = pre_post_\<sigma>\<^sub>1_\<sigma>\<^sub>2.\<sigma>\<^sub>2 oid3 oid6 oid8 oid9 oid10 oid11 oid12 oid13
+definition "\<sigma>\<^sub>t\<^sub>2 = transition_\<sigma>\<^sub>1_\<sigma>\<^sub>2.\<sigma>\<^sub>2 oid3 oid6 oid8 oid9 oid10 oid11 oid12 oid13
                   \<lceil>\<lceil>S1 (\<sigma>\<^sub>0, \<sigma>\<^sub>0)\<rceil>\<rceil> \<lceil>\<lceil>R11 (\<sigma>\<^sub>0, \<sigma>\<^sub>0)\<rceil>\<rceil> \<lceil>\<lceil>F1 (\<sigma>\<^sub>0, \<sigma>\<^sub>0)\<rceil>\<rceil> \<lceil>\<lceil>F2 (\<sigma>\<^sub>0, \<sigma>\<^sub>0)\<rceil>\<rceil>
                   \<lceil>\<lceil>\<sigma>\<^sub>2_object1 (\<sigma>\<^sub>0, \<sigma>\<^sub>0)\<rceil>\<rceil> \<lceil>\<lceil>\<sigma>\<^sub>2_object2 (\<sigma>\<^sub>0, \<sigma>\<^sub>0)\<rceil>\<rceil> \<lceil>\<lceil>\<sigma>\<^sub>2_object4 (\<sigma>\<^sub>0, \<sigma>\<^sub>0)\<rceil>\<rceil> \<lceil>\<lceil>\<sigma>\<^sub>2_object7 (\<sigma>\<^sub>0, \<sigma>\<^sub>0)\<rceil>\<rceil>"
 
-definition "s1 = state_\<sigma>\<^sub>1.\<sigma>\<^sub>1 oid3 oid4 oid5 oid6 oid7 oid8 oid9
+definition "\<sigma>\<^sub>s\<^sub>1 = state_\<sigma>\<^sub>1.\<sigma>\<^sub>1 oid3 oid4 oid5 oid6 oid7 oid8 oid9
                   \<lceil>\<lceil>S1 (\<sigma>\<^sub>0, \<sigma>\<^sub>0)\<rceil>\<rceil> \<lceil>\<lceil>C1 (\<sigma>\<^sub>0, \<sigma>\<^sub>0)\<rceil>\<rceil> \<lceil>\<lceil>C2 (\<sigma>\<^sub>0, \<sigma>\<^sub>0)\<rceil>\<rceil> \<lceil>\<lceil>R11 (\<sigma>\<^sub>0, \<sigma>\<^sub>0)\<rceil>\<rceil>
                   \<lceil>\<lceil>R21 (\<sigma>\<^sub>0, \<sigma>\<^sub>0)\<rceil>\<rceil> \<lceil>\<lceil>F1 (\<sigma>\<^sub>0, \<sigma>\<^sub>0)\<rceil>\<rceil> \<lceil>\<lceil>F2 (\<sigma>\<^sub>0, \<sigma>\<^sub>0)\<rceil>\<rceil>"
 
-definition "s2 = state_\<sigma>\<^sub>2.\<sigma>\<^sub>2 oid3 oid10 oid11 oid6 oid12 oid8 oid9 oid13
+definition "\<sigma>\<^sub>s\<^sub>2 = state_\<sigma>\<^sub>2.\<sigma>\<^sub>2 oid3 oid10 oid11 oid6 oid12 oid8 oid9 oid13
                   \<lceil>\<lceil>S1 (\<sigma>\<^sub>0, \<sigma>\<^sub>0)\<rceil>\<rceil> \<lceil>\<lceil>\<sigma>\<^sub>2_object1 (\<sigma>\<^sub>0, \<sigma>\<^sub>0)\<rceil>\<rceil> \<lceil>\<lceil>\<sigma>\<^sub>2_object2 (\<sigma>\<^sub>0, \<sigma>\<^sub>0)\<rceil>\<rceil> \<lceil>\<lceil>R11 (\<sigma>\<^sub>0, \<sigma>\<^sub>0)\<rceil>\<rceil>
                   \<lceil>\<lceil>\<sigma>\<^sub>2_object4 (\<sigma>\<^sub>0, \<sigma>\<^sub>0)\<rceil>\<rceil> \<lceil>\<lceil>F1 (\<sigma>\<^sub>0, \<sigma>\<^sub>0)\<rceil>\<rceil> \<lceil>\<lceil>F2 (\<sigma>\<^sub>0, \<sigma>\<^sub>0)\<rceil>\<rceil> \<lceil>\<lceil>\<sigma>\<^sub>2_object7 (\<sigma>\<^sub>0, \<sigma>\<^sub>0)\<rceil>\<rceil>"
 
 text{* Both formats are equivalent: *}
 
-lemma \<sigma>\<^sub>1_s1: "\<sigma>\<^sub>1 = s1"
-unfolding \<sigma>\<^sub>1_def s1_def 
- apply(subst pre_post_\<sigma>\<^sub>1_\<sigma>\<^sub>2.\<sigma>\<^sub>1_def)
+lemma \<sigma>\<^sub>t\<^sub>1_\<sigma>\<^sub>s\<^sub>1: "\<sigma>\<^sub>t\<^sub>1 = \<sigma>\<^sub>s\<^sub>1"
+unfolding \<sigma>\<^sub>t\<^sub>1_def \<sigma>\<^sub>s\<^sub>1_def 
+ apply(subst transition_\<sigma>\<^sub>1_\<sigma>\<^sub>2.\<sigma>\<^sub>1_def)
 by(rule \<sigma>\<^sub>1_\<sigma>\<^sub>2[simplified pp_\<sigma>\<^sub>1_\<sigma>\<^sub>2_def], simp)
 
 
-lemma \<sigma>\<^sub>2_s2: "\<sigma>\<^sub>2 = s2"
-unfolding \<sigma>\<^sub>2_def s2_def 
- apply(subst pre_post_\<sigma>\<^sub>1_\<sigma>\<^sub>2.\<sigma>\<^sub>2_def)
+lemma \<sigma>\<^sub>t\<^sub>2_\<sigma>\<^sub>s\<^sub>2: "\<sigma>\<^sub>t\<^sub>2 = \<sigma>\<^sub>s\<^sub>2"
+unfolding \<sigma>\<^sub>t\<^sub>2_def \<sigma>\<^sub>s\<^sub>2_def 
+ apply(subst transition_\<sigma>\<^sub>1_\<sigma>\<^sub>2.\<sigma>\<^sub>2_def)
 by(rule \<sigma>\<^sub>1_\<sigma>\<^sub>2[simplified pp_\<sigma>\<^sub>1_\<sigma>\<^sub>2_def], simp)
 
-lemma WFF_\<sigma>\<^sub>1_\<sigma>\<^sub>2: "WFF (\<sigma>\<^sub>1, \<sigma>\<^sub>2)"
-unfolding \<sigma>\<^sub>1_s1 \<sigma>\<^sub>2_s2 s1_def s2_def
- apply(rule pre_post_\<sigma>\<^sub>1_\<sigma>\<^sub>2.basic_\<sigma>\<^sub>1_\<sigma>\<^sub>2_wff)
+lemma "WFF (\<sigma>\<^sub>t\<^sub>1, \<sigma>\<^sub>t\<^sub>2)"
+unfolding \<sigma>\<^sub>t\<^sub>1_\<sigma>\<^sub>s\<^sub>1 \<sigma>\<^sub>t\<^sub>2_\<sigma>\<^sub>s\<^sub>2 \<sigma>\<^sub>s\<^sub>1_def \<sigma>\<^sub>s\<^sub>2_def
+ apply(rule transition_\<sigma>\<^sub>1_\<sigma>\<^sub>2.basic_\<sigma>\<^sub>1_\<sigma>\<^sub>2_wff)
  apply(rule \<sigma>\<^sub>1_\<sigma>\<^sub>2[simplified pp_\<sigma>\<^sub>1_\<sigma>\<^sub>2_def])
 by(simp_all add: pp_oid_\<sigma>\<^sub>1_\<sigma>\<^sub>2 pp_object_\<sigma>\<^sub>1_\<sigma>\<^sub>2 
       (* *)
@@ -344,9 +343,7 @@ text{* We wish to analyse our class model and show that the entire set of invari
 be satisfied, \ie{} there exists legal states that satisfy all constraints imposed
 by the class invariants. *}
 
-(* TODO : rename: pre_post into transition *)
-
-context pre_post_\<sigma>\<^sub>1_\<sigma>\<^sub>2
+context transition_\<sigma>\<^sub>1_\<sigma>\<^sub>2
 begin
 
 lemma Flight_at_pre_sat: "let \<tau> = (\<sigma>\<^sub>1,\<sigma>\<^sub>2) in
@@ -403,33 +400,33 @@ by(rule exI[where x = "(\<sigma>\<^sub>1,\<sigma>\<^sub>2)"], rule Flight_at_pos
 
 end
 
-context TRANS_\<sigma>\<^sub>1_\<sigma>\<^sub>2
+context TRANSITION_\<sigma>\<^sub>1_\<sigma>\<^sub>2
 begin
 lemma Flight_at_pre_sat: "\<exists> \<tau>. Flight_Aat_pre \<tau>"
 proof - 
  note S1 = \<sigma>\<^sub>1[simplified state_interpretation_\<sigma>\<^sub>1_def, of "(\<sigma>\<^sub>0,\<sigma>\<^sub>0)"]
  note PP = \<sigma>\<^sub>1_\<sigma>\<^sub>2[of "(\<sigma>\<^sub>0,\<sigma>\<^sub>0)", simplified pp_\<sigma>\<^sub>1_\<sigma>\<^sub>2_def]
 
- have F1_val: "F1 .seats@pre (s1, s2) = (\<lambda>_. \<lfloor>\<lfloor>120\<rfloor>\<rfloor>) (s1, s2)"
+ have F1_val: "F1 .seats@pre (\<sigma>\<^sub>s\<^sub>1, \<sigma>\<^sub>s\<^sub>2) = (\<lambda>_. \<lfloor>\<lfloor>120\<rfloor>\<rfloor>) (\<sigma>\<^sub>s\<^sub>1, \<sigma>\<^sub>s\<^sub>2)"
   apply(simp add: dot\<^sub>F\<^sub>l\<^sub>i\<^sub>g\<^sub>h\<^sub>t__seatsat_pre F1_def deref_oid\<^sub>F\<^sub>l\<^sub>i\<^sub>g\<^sub>h\<^sub>t_def in_pre_state_def F1\<^sub>F\<^sub>l\<^sub>i\<^sub>g\<^sub>h\<^sub>t_def oid_of_ty\<^sub>F\<^sub>l\<^sub>i\<^sub>g\<^sub>h\<^sub>t_def oid8_def)
-  apply(subst (8) s1_def, simp add: state_\<sigma>\<^sub>1.\<sigma>\<^sub>1_def[OF S1], simp add: pp_oid_\<sigma>\<^sub>1_\<sigma>\<^sub>2)
+  apply(subst (8) \<sigma>\<^sub>s\<^sub>1_def, simp add: state_\<sigma>\<^sub>1.\<sigma>\<^sub>1_def[OF S1], simp add: pp_oid_\<sigma>\<^sub>1_\<sigma>\<^sub>2)
   apply(simp add: select\<^sub>F\<^sub>l\<^sub>i\<^sub>g\<^sub>h\<^sub>t__seats_def F1_def F1\<^sub>F\<^sub>l\<^sub>i\<^sub>g\<^sub>h\<^sub>t_def)
  by(simp add: reconst_basetype_def)
 
- have F2_val: "F2 .seats@pre (s1, s2) = (\<lambda>_. \<lfloor>\<lfloor>370\<rfloor>\<rfloor>) (s1, s2)"
+ have F2_val: "F2 .seats@pre (\<sigma>\<^sub>s\<^sub>1, \<sigma>\<^sub>s\<^sub>2) = (\<lambda>_. \<lfloor>\<lfloor>370\<rfloor>\<rfloor>) (\<sigma>\<^sub>s\<^sub>1, \<sigma>\<^sub>s\<^sub>2)"
   apply(simp add: dot\<^sub>F\<^sub>l\<^sub>i\<^sub>g\<^sub>h\<^sub>t__seatsat_pre F2_def deref_oid\<^sub>F\<^sub>l\<^sub>i\<^sub>g\<^sub>h\<^sub>t_def in_pre_state_def F2\<^sub>F\<^sub>l\<^sub>i\<^sub>g\<^sub>h\<^sub>t_def oid_of_ty\<^sub>F\<^sub>l\<^sub>i\<^sub>g\<^sub>h\<^sub>t_def oid9_def)
-  apply(subst (8) s1_def, simp add: state_\<sigma>\<^sub>1.\<sigma>\<^sub>1_def[OF S1], simp add: pp_oid_\<sigma>\<^sub>1_\<sigma>\<^sub>2)
+  apply(subst (8) \<sigma>\<^sub>s\<^sub>1_def, simp add: state_\<sigma>\<^sub>1.\<sigma>\<^sub>1_def[OF S1], simp add: pp_oid_\<sigma>\<^sub>1_\<sigma>\<^sub>2)
   apply(simp add: select\<^sub>F\<^sub>l\<^sub>i\<^sub>g\<^sub>h\<^sub>t__seats_def F2_def F2\<^sub>F\<^sub>l\<^sub>i\<^sub>g\<^sub>h\<^sub>t_def)
  by(simp add: reconst_basetype_def)
 
  show ?thesis
-  apply(rule exI[where x = "(\<sigma>\<^sub>1,\<sigma>\<^sub>2)"], simp add: \<sigma>\<^sub>1_def \<sigma>\<^sub>2_def)
-  apply(rule pre_post_\<sigma>\<^sub>1_\<sigma>\<^sub>2.Flight_at_pre_sat[OF PP, simplified Let_def, THEN mp, THEN mp])
-   apply(simp add: pre_post_\<sigma>\<^sub>1_\<sigma>\<^sub>2.\<sigma>\<^sub>1_def[OF PP] pre_post_\<sigma>\<^sub>1_\<sigma>\<^sub>2.\<sigma>\<^sub>2_def[OF PP], fold s1_def, fold s2_def)
+  apply(rule exI[where x = "(\<sigma>\<^sub>t\<^sub>1,\<sigma>\<^sub>t\<^sub>2)"], simp add: \<sigma>\<^sub>t\<^sub>1_def \<sigma>\<^sub>t\<^sub>2_def)
+  apply(rule transition_\<sigma>\<^sub>1_\<sigma>\<^sub>2.Flight_at_pre_sat[OF PP, simplified Let_def, THEN mp, THEN mp])
+   apply(simp add: transition_\<sigma>\<^sub>1_\<sigma>\<^sub>2.\<sigma>\<^sub>1_def[OF PP] transition_\<sigma>\<^sub>1_\<sigma>\<^sub>2.\<sigma>\<^sub>2_def[OF PP], fold \<sigma>\<^sub>s\<^sub>1_def, fold \<sigma>\<^sub>s\<^sub>2_def)
    apply(simp add: OclValid_def)
   apply(subst OclLess\<^sub>I\<^sub>n\<^sub>t\<^sub>e\<^sub>g\<^sub>e\<^sub>r.cp0, simp add: F1_val OclInt0_def OclLess\<^sub>I\<^sub>n\<^sub>t\<^sub>e\<^sub>g\<^sub>e\<^sub>r_def)
 
-  apply(simp add: pre_post_\<sigma>\<^sub>1_\<sigma>\<^sub>2.\<sigma>\<^sub>1_def[OF PP] pre_post_\<sigma>\<^sub>1_\<sigma>\<^sub>2.\<sigma>\<^sub>2_def[OF PP], fold s1_def, fold s2_def)
+  apply(simp add: transition_\<sigma>\<^sub>1_\<sigma>\<^sub>2.\<sigma>\<^sub>1_def[OF PP] transition_\<sigma>\<^sub>1_\<sigma>\<^sub>2.\<sigma>\<^sub>2_def[OF PP], fold \<sigma>\<^sub>s\<^sub>1_def, fold \<sigma>\<^sub>s\<^sub>2_def)
   apply(simp add: OclValid_def)
   apply(subst OclLess\<^sub>I\<^sub>n\<^sub>t\<^sub>e\<^sub>g\<^sub>e\<^sub>r.cp0, simp add: F2_val OclInt0_def OclLess\<^sub>I\<^sub>n\<^sub>t\<^sub>e\<^sub>g\<^sub>e\<^sub>r_def)
  done
@@ -440,34 +437,34 @@ proof -
  note S2 = \<sigma>\<^sub>2[simplified state_interpretation_\<sigma>\<^sub>2_def, of "(\<sigma>\<^sub>0,\<sigma>\<^sub>0)"]
  note PP = \<sigma>\<^sub>1_\<sigma>\<^sub>2[of "(\<sigma>\<^sub>0,\<sigma>\<^sub>0)", simplified pp_\<sigma>\<^sub>1_\<sigma>\<^sub>2_def]
 
- have F1_val: "F1 .seats (s1, s2) = (\<lambda>_. \<lfloor>\<lfloor>120\<rfloor>\<rfloor>) (s1, s2)"
+ have F1_val: "F1 .seats (\<sigma>\<^sub>s\<^sub>1, \<sigma>\<^sub>s\<^sub>2) = (\<lambda>_. \<lfloor>\<lfloor>120\<rfloor>\<rfloor>) (\<sigma>\<^sub>s\<^sub>1, \<sigma>\<^sub>s\<^sub>2)"
   apply(simp add: dot\<^sub>F\<^sub>l\<^sub>i\<^sub>g\<^sub>h\<^sub>t__seats F1_def deref_oid\<^sub>F\<^sub>l\<^sub>i\<^sub>g\<^sub>h\<^sub>t_def in_post_state_def F1\<^sub>F\<^sub>l\<^sub>i\<^sub>g\<^sub>h\<^sub>t_def oid_of_ty\<^sub>F\<^sub>l\<^sub>i\<^sub>g\<^sub>h\<^sub>t_def oid8_def)
-  apply(subst (8) s2_def, simp add: state_\<sigma>\<^sub>2.\<sigma>\<^sub>2_def[OF S2], simp add: pp_oid_\<sigma>\<^sub>1_\<sigma>\<^sub>2)
+  apply(subst (8) \<sigma>\<^sub>s\<^sub>2_def, simp add: state_\<sigma>\<^sub>2.\<sigma>\<^sub>2_def[OF S2], simp add: pp_oid_\<sigma>\<^sub>1_\<sigma>\<^sub>2)
   apply(simp add: select\<^sub>F\<^sub>l\<^sub>i\<^sub>g\<^sub>h\<^sub>t__seats_def F1_def F1\<^sub>F\<^sub>l\<^sub>i\<^sub>g\<^sub>h\<^sub>t_def)
  by(simp add: reconst_basetype_def)
 
- have F2_val: "F2 .seats (s1, s2) = (\<lambda>_. \<lfloor>\<lfloor>370\<rfloor>\<rfloor>) (s1, s2)"
+ have F2_val: "F2 .seats (\<sigma>\<^sub>s\<^sub>1, \<sigma>\<^sub>s\<^sub>2) = (\<lambda>_. \<lfloor>\<lfloor>370\<rfloor>\<rfloor>) (\<sigma>\<^sub>s\<^sub>1, \<sigma>\<^sub>s\<^sub>2)"
   apply(simp add: dot\<^sub>F\<^sub>l\<^sub>i\<^sub>g\<^sub>h\<^sub>t__seats F2_def deref_oid\<^sub>F\<^sub>l\<^sub>i\<^sub>g\<^sub>h\<^sub>t_def in_post_state_def F2\<^sub>F\<^sub>l\<^sub>i\<^sub>g\<^sub>h\<^sub>t_def oid_of_ty\<^sub>F\<^sub>l\<^sub>i\<^sub>g\<^sub>h\<^sub>t_def oid8_def)
-  apply(subst (8) s2_def, simp add: state_\<sigma>\<^sub>2.\<sigma>\<^sub>2_def[OF S2], simp add: pp_oid_\<sigma>\<^sub>1_\<sigma>\<^sub>2)
+  apply(subst (8) \<sigma>\<^sub>s\<^sub>2_def, simp add: state_\<sigma>\<^sub>2.\<sigma>\<^sub>2_def[OF S2], simp add: pp_oid_\<sigma>\<^sub>1_\<sigma>\<^sub>2)
   apply(simp add: select\<^sub>F\<^sub>l\<^sub>i\<^sub>g\<^sub>h\<^sub>t__seats_def F2_def F2\<^sub>F\<^sub>l\<^sub>i\<^sub>g\<^sub>h\<^sub>t_def)
  by(simp add: reconst_basetype_def)
 
  show ?thesis
-  apply(rule exI[where x = "(\<sigma>\<^sub>1,\<sigma>\<^sub>2)"], simp add: \<sigma>\<^sub>1_def \<sigma>\<^sub>2_def)
-  apply(rule pre_post_\<sigma>\<^sub>1_\<sigma>\<^sub>2.Flight_at_post_sat[OF PP, simplified Let_def, THEN mp, THEN mp])
-   apply(simp add: pre_post_\<sigma>\<^sub>1_\<sigma>\<^sub>2.\<sigma>\<^sub>1_def[OF PP] pre_post_\<sigma>\<^sub>1_\<sigma>\<^sub>2.\<sigma>\<^sub>2_def[OF PP], fold s1_def, fold s2_def)
+  apply(rule exI[where x = "(\<sigma>\<^sub>t\<^sub>1,\<sigma>\<^sub>t\<^sub>2)"], simp add: \<sigma>\<^sub>t\<^sub>1_def \<sigma>\<^sub>t\<^sub>2_def)
+  apply(rule transition_\<sigma>\<^sub>1_\<sigma>\<^sub>2.Flight_at_post_sat[OF PP, simplified Let_def, THEN mp, THEN mp])
+   apply(simp add: transition_\<sigma>\<^sub>1_\<sigma>\<^sub>2.\<sigma>\<^sub>1_def[OF PP] transition_\<sigma>\<^sub>1_\<sigma>\<^sub>2.\<sigma>\<^sub>2_def[OF PP], fold \<sigma>\<^sub>s\<^sub>1_def, fold \<sigma>\<^sub>s\<^sub>2_def)
    apply(simp add: OclValid_def)
   apply(subst OclLess\<^sub>I\<^sub>n\<^sub>t\<^sub>e\<^sub>g\<^sub>e\<^sub>r.cp0, simp add: F1_val OclInt0_def OclLess\<^sub>I\<^sub>n\<^sub>t\<^sub>e\<^sub>g\<^sub>e\<^sub>r_def)
 
-  apply(simp add: pre_post_\<sigma>\<^sub>1_\<sigma>\<^sub>2.\<sigma>\<^sub>1_def[OF PP] pre_post_\<sigma>\<^sub>1_\<sigma>\<^sub>2.\<sigma>\<^sub>2_def[OF PP], fold s1_def, fold s2_def)
+  apply(simp add: transition_\<sigma>\<^sub>1_\<sigma>\<^sub>2.\<sigma>\<^sub>1_def[OF PP] transition_\<sigma>\<^sub>1_\<sigma>\<^sub>2.\<sigma>\<^sub>2_def[OF PP], fold \<sigma>\<^sub>s\<^sub>1_def, fold \<sigma>\<^sub>s\<^sub>2_def)
   apply(simp add: OclValid_def)
   apply(subst OclLess\<^sub>I\<^sub>n\<^sub>t\<^sub>e\<^sub>g\<^sub>e\<^sub>r.cp0, simp add: F2_val OclInt0_def OclLess\<^sub>I\<^sub>n\<^sub>t\<^sub>e\<^sub>g\<^sub>e\<^sub>r_def)
  done
 qed
 end
 
-thm TRANS_\<sigma>\<^sub>1_\<sigma>\<^sub>2.Flight_at_pre_sat[simplified Flight_Aat_pre_def]
-thm TRANS_\<sigma>\<^sub>1_\<sigma>\<^sub>2.Flight_at_post_sat[simplified Flight_A_def]
+thm TRANSITION_\<sigma>\<^sub>1_\<sigma>\<^sub>2.Flight_at_pre_sat[simplified Flight_Aat_pre_def]
+thm TRANSITION_\<sigma>\<^sub>1_\<sigma>\<^sub>2.Flight_at_post_sat[simplified Flight_A_def]
 
 Context r: Reservation
   Inv A : "\<zero> <\<^sub>i\<^sub>n\<^sub>t (r .id)"
